src/theory/bir/bir_valuesScript.sml
@@ -11,22 +11,34 @@ val bir_imm_ss = rewrites ((type_rws ``:bir_imm_t``) @ (type_rws ``:bir_immtype_
 (*  Datatypes                                                                *)
 (* ------------------------------------------------------------------------- *)
 
+(* Known BIR values *)
+val _ = Datatype `bir_val_k_t =
+    BKVal_Imm bir_imm_t
+  | BKVal_Mem bir_immtype_t (* Address type *)
+             bir_immtype_t (* Value type *)
+             (num |-> num) (* Memory map *)
+`;
+
+(* Generic BIR values *)
 val _ = Datatype `bir_val_t =
     BVal_Unknown
-  | BVal_Imm bir_imm_t
-  | BVal_Mem bir_immtype_t (*Addr-Type*) bir_immtype_t (* value-type *) (num |-> num)
+  | BVal_Known bir_val_k_t
 `;
 
 
 val _ = Datatype `bir_type_t =
     BType_Imm bir_immtype_t
-  | BType_Mem bir_immtype_t (* Addr-Type *) bir_immtype_t (* Value-Type *)
+  | BType_Mem bir_immtype_t (* Address type *)
+              bir_immtype_t (* Value type *)
 `;
 
 val BType_Bool_def = Define `BType_Bool = BType_Imm Bit1`;
 
 
-val bir_val_ss = rewrites (type_rws ``:bir_val_t``);
+val bir_val_ss =
+  rewrites ((type_rws ``:bir_val_k_t``) @
+	      (type_rws ``:bir_val_t``)
+  );
 val bir_type_ss = rewrites (type_rws ``:bir_type_t``);
 
 
@@ -34,114 +46,334 @@ val bir_type_ss = rewrites (type_rws ``:bir_type_t``);
 (*  Checkers for Values                                                      *)
 (* ------------------------------------------------------------------------- *)
 
-val bir_val_is_Unknown_def = Define `bir_val_is_Unknown v = (v = BVal_Unknown)`;
-val bir_val_is_Imm_def = Define `bir_val_is_Imm v = ?b. (v = BVal_Imm b)`;
-val bir_val_is_Imm_s_def = Define `bir_val_is_Imm_s s v = ?n. (v = BVal_Imm (n2bs n s))`;
-val bir_val_is_Bool_def = Define `bir_val_is_Bool = bir_val_is_Imm_s Bit1`;
-val bir_val_is_Mem_def = Define `bir_val_is_Mem v = ?at vt mmap. (v = BVal_Mem at vt mmap)`;
+(* Generic values *)
+val bir_val_is_Unknown_def = Define `
+  bir_val_is_Unknown v = (v = BVal_Unknown)
+`;
+val bir_val_is_Known_def = Define `
+  bir_val_is_Known v = ?kv. (v = BVal_Known kv)
+`;
+val bir_val_is_Imm_def = Define `
+  bir_val_is_Imm kv = ?b. (kv = BVal_Known (BKVal_Imm b))
+`;
+val bir_val_is_Imm_s_def = Define `
+  bir_val_is_Imm_s s kv =
+    ?n. (kv = BVal_Known (BKVal_Imm (n2bs n s)))
+`;
+val bir_val_is_Bool_def = Define `
+  bir_val_is_Bool = bir_val_is_Imm_s Bit1
+`;
+val bir_val_is_Mem_def = Define `
+  bir_val_is_Mem kv =
+    ?at vt mmap. (kv = BVal_Known (BKVal_Mem at vt mmap))
+`;
 
-val bir_val_checker_DEFS = save_thm ("bir_val_checker_DEFS", LIST_CONJ [
-  bir_val_is_Unknown_def, bir_val_is_Imm_def, bir_val_is_Imm_s_def,
-  bir_val_is_Bool_def, bir_val_is_Mem_def]);
+(* Known values *)
+val bir_kval_is_Imm_def = Define `
+  bir_kval_is_Imm kv = ?b. (kv = BKVal_Imm b)
+`;
+val bir_kval_is_Imm_s_def = Define `
+  bir_kval_is_Imm_s s kv = ?n. (kv = BKVal_Imm (n2bs n s))
+`;
+val bir_kval_is_Bool_def = Define `
+  bir_kval_is_Bool = bir_kval_is_Imm_s Bit1
+`;
+val bir_kval_is_Mem_def = Define `
+  bir_kval_is_Mem kv = ?at vt mmap. (kv = BKVal_Mem at vt mmap)
+`;
+
+val bir_val_checker_DEFS =
+  save_thm ("bir_val_checker_DEFS",
+    LIST_CONJ [
+      bir_val_is_Unknown_def,
+      bir_val_is_Known_def,
+      bir_val_is_Imm_def,
+      bir_val_is_Imm_s_def,
+      bir_val_is_Bool_def,
+      bir_val_is_Mem_def,
+      bir_kval_is_Imm_def,
+      bir_kval_is_Imm_s_def,
+      bir_kval_is_Bool_def,
+      bir_kval_is_Mem_def
+    ]
+);
 
 
-val bir_val_is_Imm_s_ALT_DEF = store_thm ("bir_val_is_Imm_s_ALT_DEF",
-``!s v. bir_val_is_Imm_s s v <=>
-  (?b. (v = BVal_Imm b) /\ (type_of_bir_imm b = s))``,
+val bir_val_is_Imm_s_ALT_DEF =
+  store_thm ("bir_val_is_Imm_s_ALT_DEF",
+  ``!s v. bir_val_is_Imm_s s v <=>
+    (?b.
+      (v = BVal_Known (BKVal_Imm b)) /\
+      (type_of_bir_imm b = s)
+    )``,
 
 Cases_on `v` >> (
-  SIMP_TAC (std_ss ++ bir_val_ss) [bir_val_is_Imm_s_def,
+  SIMP_TAC (std_ss++bir_val_ss) [bir_val_is_Imm_s_def,
     type_of_bir_imm_n2bs_INTRO]
-));
+) >>
+METIS_TAC []
+);
+
+val bir_kval_is_Imm_s_ALT_DEF =
+  store_thm ("bir_kval_is_Imm_s_ALT_DEF",
+  ``!s v. bir_kval_is_Imm_s s v <=>
+    (?b. (v = BKVal_Imm b) /\ (type_of_bir_imm b = s))``,
+
+Cases_on `v` >> (
+  SIMP_TAC (std_ss++bir_val_ss) [bir_kval_is_Imm_s_def,
+    type_of_bir_imm_n2bs_INTRO]
+)
+);
 
 
 val bir_val_checker_REWRS = store_thm ("bir_val_checker_REWRS",
   ``bir_val_is_Unknown BVal_Unknown /\
-    (!b. ~bir_val_is_Unknown (BVal_Imm b)) /\
-    (!at vt mmap. ~(bir_val_is_Unknown (BVal_Mem at vt mmap))) /\
+    (!kv. ~bir_val_is_Unknown (BVal_Known kv)) /\
+
+    (~bir_val_is_Known BVal_Unknown) /\
+    (!kv. bir_val_is_Known (BVal_Known kv)) /\
 
     ~(bir_val_is_Imm BVal_Unknown) /\
-    (!b. bir_val_is_Imm (BVal_Imm b)) /\
-    (!at vt mmap. ~(bir_val_is_Imm (BVal_Mem at vt mmap))) /\
-
-    ~(bir_val_is_Mem BVal_Unknown) /\
-    (!b. ~(bir_val_is_Mem (BVal_Imm b))) /\
-    (!at vt mmap. (bir_val_is_Mem (BVal_Mem at vt mmap))) /\
+    (!b. bir_val_is_Imm (BVal_Known (BKVal_Imm b))) /\
+    (!at vt mmap.
+       ~(bir_val_is_Imm (BVal_Known (BKVal_Mem at vt mmap)))
+    ) /\
 
     (!s. ~(bir_val_is_Imm_s s BVal_Unknown)) /\
-    (!s b. bir_val_is_Imm_s s (BVal_Imm b) <=> (type_of_bir_imm b = s)) /\
-    (!s at vt mmap. ~(bir_val_is_Imm_s s (BVal_Mem at vt mmap))) /\
+    (!s b. bir_val_is_Imm_s s (BVal_Known (BKVal_Imm b)) <=>
+           (type_of_bir_imm b = s)
+    ) /\
+    (!s at vt mmap.
+       ~(bir_val_is_Imm_s s (BVal_Known (BKVal_Mem at vt mmap)))
+    ) /\
 
     (~(bir_val_is_Bool BVal_Unknown)) /\
-    (!b. bir_val_is_Bool (BVal_Imm b) <=> (type_of_bir_imm b = Bit1)) /\
-    (!at vt mmap. ~(bir_val_is_Bool (BVal_Mem at vt mmap)))``,
+    (!b. bir_val_is_Bool (BVal_Known (BKVal_Imm b)) <=>
+         (type_of_bir_imm b = Bit1)
+    ) /\
+    (!at vt mmap.
+       ~(bir_val_is_Bool (BVal_Known (BKVal_Mem at vt mmap)))
+    ) /\
 
+    ~(bir_val_is_Mem BVal_Unknown) /\
+    (!b. ~(bir_val_is_Mem (BVal_Known (BKVal_Imm b)))) /\
+    (!at vt mmap.
+       (bir_val_is_Mem (BVal_Known (BKVal_Mem at vt mmap)))
+    ) /\
 
-  REWRITE_TAC[bir_val_is_Imm_s_ALT_DEF, bir_val_is_Bool_def] >>
-  SIMP_TAC (std_ss ++ bir_val_ss) [bir_val_checker_DEFS]);
+    (!b. bir_kval_is_Imm (BKVal_Imm b)) /\
+    (!at vt mmap. ~(bir_kval_is_Imm (BKVal_Mem at vt mmap))) /\
+
+    (!b. ~(bir_kval_is_Mem (BKVal_Imm b))) /\
+    (!at vt mmap. (bir_kval_is_Mem (BKVal_Mem at vt mmap))) /\
+
+    (!s b. bir_kval_is_Imm_s s (BKVal_Imm b) <=>
+           (type_of_bir_imm b = s)
+    ) /\
+    (!s at vt mmap. ~(bir_kval_is_Imm_s s (BKVal_Mem at vt mmap))) /\
+
+    (!b. bir_kval_is_Bool (BKVal_Imm b) <=>
+         (type_of_bir_imm b = Bit1)
+    ) /\
+    (!at vt mmap. ~(bir_kval_is_Bool (BKVal_Mem at vt mmap)))``,
+
+REWRITE_TAC[bir_val_is_Imm_s_ALT_DEF, bir_kval_is_Imm_s_ALT_DEF,
+            bir_val_is_Bool_def, bir_kval_is_Bool_def] >>
+SIMP_TAC (std_ss++bir_val_ss) [bir_val_checker_DEFS]
+);
 
 
 val bir_val_is_Imm_s_IMPL = store_thm ("bir_val_is_Imm_s_IMPL",
   ``!s v. bir_val_is_Imm_s s v ==> bir_val_is_Imm v``,
-SIMP_TAC (std_ss++bir_val_ss) [bir_val_is_Imm_def, bir_val_is_Imm_s_def,
-  GSYM LEFT_FORALL_IMP_THM]);
+
+SIMP_TAC (std_ss++bir_val_ss) [bir_val_is_Imm_def,
+                               bir_val_is_Imm_s_def,
+                               GSYM LEFT_FORALL_IMP_THM]
+);
+
+val bir_kval_is_Imm_s_IMPL = store_thm ("bir_kval_is_Imm_s_IMPL",
+  ``!s v. bir_kval_is_Imm_s s v ==> bir_kval_is_Imm v``,
+
+SIMP_TAC (std_ss++bir_val_ss) [bir_kval_is_Imm_def,
+                               bir_kval_is_Imm_s_def,
+                               GSYM LEFT_FORALL_IMP_THM]
+);
 
 val bir_val_is_Bool_IMPL = store_thm ("bir_val_is_Bool_IMPL",
   ``!v. bir_val_is_Bool v ==> bir_val_is_Imm v``,
-SIMP_TAC (std_ss++bir_val_ss) [bir_val_is_Imm_def, bir_val_is_Bool_def,
-  bir_val_is_Imm_s_def, GSYM LEFT_FORALL_IMP_THM]);
 
+SIMP_TAC (std_ss++bir_val_ss) [bir_val_is_Imm_def,
+                               bir_val_is_Bool_def,
+                               bir_val_is_Imm_s_def,
+                               GSYM LEFT_FORALL_IMP_THM]
+);
+
+val bir_kval_is_Bool_IMPL = store_thm ("bir_kval_is_Bool_IMPL",
+  ``!v. bir_kval_is_Bool v ==> bir_kval_is_Imm v``,
+
+SIMP_TAC (std_ss++bir_val_ss) [bir_kval_is_Imm_def,
+                               bir_kval_is_Bool_def,
+                               bir_kval_is_Imm_s_def,
+                               GSYM LEFT_FORALL_IMP_THM]
+);
 
 
 (* ------------------------------------------------------------------------- *)
 (*  Boolean Values                                                           *)
 (* ------------------------------------------------------------------------- *)
 
+(* TODO: Make bir_dest_bool_val defined in terms of
+ * bir_dest_bool_kval? *)
 val bir_dest_bool_val_def = Define `
-  (bir_dest_bool_val (BVal_Imm (Imm1 w)) = SOME (w = 1w)) /\
-  (bir_dest_bool_val _ = NONE)`
+  (bir_dest_bool_val (BVal_Known (BKVal_Imm (Imm1 w))) =
+    SOME (w = 1w)
+  ) /\
+  (bir_dest_bool_val _ = NONE)
+`;
 
-val bir_dest_bool_val_EQ_SOME = store_thm ("bir_dest_bool_val_EQ_SOME",
-  ``!v b. (bir_dest_bool_val v = SOME b) <=> (v = BVal_Imm (bool2b b))``,
-Cases >> SIMP_TAC (std_ss++bir_val_ss) [bir_dest_bool_val_def] >>
-rename1 `BVal_Imm i` >>
-Cases_on `i` >> SIMP_TAC (std_ss++bir_imm_ss) [bir_dest_bool_val_def, bool2b_NEQ_IMM_ELIMS] >>
-SIMP_TAC (std_ss++bir_imm_ss) [bool2b_def] >>
-Cases_on `b'` >> SIMP_TAC std_ss [bool2w_def] >>
-METIS_TAC[word1_dichotomy, word1_distinct]);
+val bir_dest_bool_kval_def = Define `
+  (bir_dest_bool_kval (BKVal_Imm (Imm1 w)) = SOME (w = 1w)) /\
+  (bir_dest_bool_kval _ = NONE)
+`;
 
-val bir_dest_bool_val_EQ_NONE = store_thm ("bir_dest_bool_val_EQ_NONE",
+val bir_dest_bool_val_EQ_SOME =
+  store_thm ("bir_dest_bool_val_EQ_SOME",
+  ``!v b. (bir_dest_bool_val v = SOME b) <=>
+          (v = (BVal_Known (BKVal_Imm (bool2b b))))``,
+
+Cases >| [
+  SIMP_TAC (std_ss++bir_val_ss) [bir_dest_bool_val_def],
+
+  Cases_on `b` >| [
+    rename1 `BKVal_Imm i` >>
+    Cases_on `i` >> (
+      SIMP_TAC (std_ss++bir_imm_ss++bir_val_ss)
+               [bir_dest_bool_val_def, bool2b_NEQ_IMM_ELIMS,
+                bool2b_def]
+    ) >>
+    Cases_on `b` >> (
+      SIMP_TAC (std_ss++bir_val_ss) [bool2w_def] >>
+      METIS_TAC [word1_dichotomy, word1_distinct]
+    ),
+   
+    SIMP_TAC (std_ss++bir_val_ss) [bir_dest_bool_val_def]
+  ]
+]
+);
+
+val bir_dest_bool_kval_EQ_SOME =
+  store_thm ("bir_dest_bool_kval_EQ_SOME",
+  ``!v b. (bir_dest_bool_kval v = SOME b) <=>
+          (v = BKVal_Imm (bool2b b))``,
+
+Cases >| [
+  Cases_on `b` >> (
+    SIMP_TAC (std_ss++bir_imm_ss++bir_val_ss)
+	     [bir_dest_bool_kval_def, bool2b_NEQ_IMM_ELIMS,
+	      bool2b_def]
+  ) >>
+  Cases_on `b` >> (
+    SIMP_TAC (std_ss++bir_val_ss) [bool2w_def] >>
+    METIS_TAC [word1_dichotomy, word1_distinct]
+  ),
+
+  SIMP_TAC (std_ss++bir_val_ss) [bir_dest_bool_kval_def]
+]
+);
+
+val bir_dest_bool_val_EQ_NONE =
+  store_thm ("bir_dest_bool_val_EQ_NONE",
   ``!v. (bir_dest_bool_val v = NONE) <=> ~(bir_val_is_Bool v)``,
-Cases >> SIMP_TAC std_ss [bir_val_checker_REWRS, bir_dest_bool_val_def] >>
-Cases_on `b` >> SIMP_TAC (std_ss++bir_imm_ss) [bir_val_checker_REWRS, bir_dest_bool_val_def,
-  type_of_bir_imm_def]);
 
-val bir_dest_bool_val_bool2b = store_thm ("bir_dest_bool_val_bool2b",
-  ``bir_dest_bool_val (BVal_Imm (bool2b b)) = SOME b``,
-SIMP_TAC (std_ss++boolSimps.LIFT_COND_ss++wordsLib.WORD_ss) [
-  bool2b_def, bool2w_def, bir_dest_bool_val_def]);
+Cases >> (
+  SIMP_TAC std_ss [bir_val_checker_REWRS, bir_dest_bool_val_def]
+) >>
+Cases_on `b` >| [
+  Cases_on `b'` >> (
+    SIMP_TAC (std_ss++bir_imm_ss) [bir_val_checker_REWRS,
+				   bir_dest_bool_val_def,
+				   type_of_bir_imm_def]
+  ),
+
+  SIMP_TAC std_ss [bir_val_checker_REWRS, bir_dest_bool_val_def]
+]
+);
+
+val bir_dest_bool_kval_EQ_NONE =
+  store_thm ("bir_dest_bool_kval_EQ_NONE",
+  ``!v. (bir_dest_bool_kval v = NONE) <=> ~(bir_kval_is_Bool v)``,
+
+Cases >> (
+  SIMP_TAC std_ss [bir_val_checker_REWRS, bir_dest_bool_kval_def]
+) >>
+Cases_on `b` >> (
+  SIMP_TAC (std_ss++bir_imm_ss) [bir_val_checker_REWRS,
+				 bir_dest_bool_kval_def,
+				 type_of_bir_imm_def]
+)
+);
+
+val bir_dest_bool_val_bool2b =
+  store_thm ("bir_dest_bool_val_bool2b",
+  ``!b.
+      bir_dest_bool_val (BVal_Known (BKVal_Imm (bool2b b))) =
+        SOME b``,
+
+SIMP_TAC (std_ss++boolSimps.LIFT_COND_ss++wordsLib.WORD_ss)
+         [bool2b_def, bool2w_def, bir_dest_bool_val_def]
+);
+
+val bir_dest_bool_kval_bool2b =
+  store_thm ("bir_dest_bool_kval_bool2b",
+  ``!b. bir_dest_bool_kval (BKVal_Imm (bool2b b)) = SOME b``,
+
+SIMP_TAC (std_ss++boolSimps.LIFT_COND_ss++wordsLib.WORD_ss)
+         [bool2b_def, bool2w_def, bir_dest_bool_kval_def]
+);
 
 (* ------------------------------------------------------------------------- *)
 (*  Some basic typing                                                        *)
 (* ------------------------------------------------------------------------- *)
 
+val type_of_bir_kval_def = Define `
+  (type_of_bir_kval (BKVal_Imm imm) =
+    BType_Imm (type_of_bir_imm imm)
+  ) /\
+  (type_of_bir_kval (BKVal_Mem at vt _) = BType_Mem at vt)
+`;
+
 val type_of_bir_val_def = Define `
   (type_of_bir_val BVal_Unknown = NONE) /\
-  (type_of_bir_val (BVal_Imm imm) = SOME (BType_Imm (type_of_bir_imm imm))) /\
-  (type_of_bir_val (BVal_Mem at vt _) = SOME (BType_Mem at vt))`;
-
-val bir_type_is_Imm_def = Define `bir_type_is_Imm ty = (?s. ty = BType_Imm s)`;
-val bir_type_is_Imm_s_def = Define `bir_type_is_Imm_s s ty = (ty = BType_Imm s)`
-val bir_type_is_Bool_def = Define `bir_type_is_Bool ty = (ty = BType_Imm Bit1)`
-val bir_type_is_Mem_def = Define `bir_type_is_Mem ty = (?at vt. ty = BType_Mem at vt)`;
-
-val bir_type_checker_DEFS = save_thm ("bir_type_checker_DEFS", LIST_CONJ [
-  bir_type_is_Imm_def, bir_type_is_Imm_s_def,
-  bir_type_is_Bool_def, bir_type_is_Mem_def]);
+  (!kv. type_of_bir_val (BVal_Known kv) =
+    SOME (type_of_bir_kval kv)
+  )
+`;
 
 
-val bir_type_checker_REWRS = store_thm ("bir_type_checker_REWRS", ``
-    (!b. bir_type_is_Imm (BType_Imm b)) /\
+val bir_type_is_Imm_def = Define `
+  bir_type_is_Imm ty = (?s. ty = BType_Imm s)
+`;
+val bir_type_is_Imm_s_def = Define `
+  bir_type_is_Imm_s s ty = (ty = BType_Imm s)
+`;
+val bir_type_is_Bool_def = Define `
+  bir_type_is_Bool ty = (ty = BType_Imm Bit1)
+`;
+val bir_type_is_Mem_def = Define `
+  bir_type_is_Mem ty = (?at vt. ty = BType_Mem at vt)
+`;
+
+val bir_type_checker_DEFS =
+  save_thm ("bir_type_checker_DEFS",
+    LIST_CONJ [
+      bir_type_is_Imm_def, bir_type_is_Imm_s_def,
+      bir_type_is_Bool_def, bir_type_is_Mem_def
+    ]
+);
+
+
+val bir_type_checker_REWRS = store_thm ("bir_type_checker_REWRS",
+  ``(!b. bir_type_is_Imm (BType_Imm b)) /\
     (!at vt. ~(bir_type_is_Imm (BType_Mem at vt))) /\
 
     (!b. ~(bir_type_is_Mem (BType_Imm b))) /\
@@ -155,42 +387,84 @@ val bir_type_checker_REWRS = store_thm ("bir_type_checker_REWRS", ``
     (!b. bir_type_is_Bool (BType_Imm b) <=> (b = Bit1)) /\
     (!at vt. ~(bir_type_is_Bool (BType_Mem at vt)))``,
 
-  SIMP_TAC (std_ss ++ bir_type_ss) [bir_type_checker_DEFS, BType_Bool_def]);
+SIMP_TAC (std_ss++bir_type_ss) [bir_type_checker_DEFS,
+                                BType_Bool_def]
+);
 
 
 val bir_type_is_Imm_s_IMPL = store_thm ("bir_type_is_Imm_s_IMPL",
   ``!s v. bir_type_is_Imm_s s v ==> bir_type_is_Imm v``,
-SIMP_TAC (std_ss++bir_type_ss) [bir_type_is_Imm_def, bir_type_is_Imm_s_def]);
+
+SIMP_TAC (std_ss++bir_type_ss) [bir_type_is_Imm_def,
+                                bir_type_is_Imm_s_def]
+);
 
 
 val bir_type_is_Bool_IMPL = store_thm ("bir_type_is_Bool_IMPL",
   ``!v. bir_type_is_Bool v ==> bir_type_is_Imm v``,
-SIMP_TAC (std_ss++bir_type_ss) [bir_type_is_Imm_def, bir_type_is_Bool_def]);
+
+SIMP_TAC (std_ss++bir_type_ss) [bir_type_is_Imm_def,
+                                bir_type_is_Bool_def]
+);
 
 
-val type_of_bir_val_EQ_ELIMS = store_thm ("type_of_bir_val_EQ_ELIMS",
+val type_of_bir_val_EQ_ELIMS =
+  store_thm ("type_of_bir_val_EQ_ELIMS",
   ``(!v. (type_of_bir_val v = NONE) <=> (v = BVal_Unknown)) /\
     (!v ty. (type_of_bir_val v = SOME (BType_Imm ty)) <=>
-            (?i. (type_of_bir_imm i = ty) /\ (v = BVal_Imm i))) /\
+            (?i. (type_of_bir_imm i = ty) /\
+                 (v = BVal_Known (BKVal_Imm i))
+            )
+    ) /\
     (!v aty vty. (type_of_bir_val v = SOME (BType_Mem aty vty)) <=>
-            (?f. (v = BVal_Mem aty vty f)))``,
-REPEAT CONJ_TAC >> Cases >> (
-  SIMP_TAC (std_ss++bir_val_ss++bir_type_ss) [type_of_bir_val_def]
-));
+                 (?f. (v = BVal_Known (BKVal_Mem aty vty f))
+                 )
+    )``,
+
+REPEAT CONJ_TAC >- (
+  Cases >> (
+    SIMP_TAC (std_ss++bir_val_ss)
+             [type_of_bir_val_def]
+  )
+) >> (
+  Cases >> (
+    SIMP_TAC (std_ss++bir_val_ss)
+	     [type_of_bir_val_def]
+  ) >>
+  Cases_on `b` >> (
+    SIMP_TAC (std_ss++bir_val_ss++bir_type_ss)
+	     [type_of_bir_val_def,
+	      type_of_bir_kval_def]
+  )
+)
+);
 
 
-val bir_val_checker_TO_type_of = store_thm ("bir_val_checker_TO_type_of",
+val bir_val_checker_TO_type_of =
+  store_thm ("bir_val_checker_TO_type_of",
   ``(!v. (bir_val_is_Unknown v) <=> (type_of_bir_val v = NONE)) /\
-    (!v ty. (bir_val_is_Imm_s ty v) <=> (type_of_bir_val v = SOME (BType_Imm ty))) /\
-    (!v. (bir_val_is_Imm v) <=> (?ty. type_of_bir_val v = SOME (BType_Imm ty))) /\
-    (!v. (bir_val_is_Bool v) <=> (type_of_bir_val v = SOME BType_Bool)) /\
+    (!v ty. (bir_val_is_Imm_s ty v) <=>
+            (type_of_bir_val v = SOME (BType_Imm ty))
+    ) /\
+    (!v. (bir_val_is_Imm v) <=>
+         (?ty. type_of_bir_val v = SOME (BType_Imm ty))
+    ) /\
+    (!v. (bir_val_is_Bool v) <=>
+         (type_of_bir_val v = SOME BType_Bool)
+    ) /\
     (!v. (bir_val_is_Mem v <=>
-         (?aty vty. type_of_bir_val v = SOME (BType_Mem aty vty))))``,
+         (?aty vty. type_of_bir_val v = SOME (BType_Mem aty vty)))
+    )``,
 
-SIMP_TAC (std_ss++boolSimps.CONJ_ss) [type_of_bir_val_EQ_ELIMS, BType_Bool_def, bir_val_is_Bool_def,
-  bir_val_is_Imm_s_ALT_DEF, bir_val_is_Imm_def, bir_val_is_Unknown_def,
-  bir_val_is_Mem_def] >>
-METIS_TAC[]);
+SIMP_TAC (std_ss++boolSimps.CONJ_ss) [type_of_bir_val_EQ_ELIMS,
+                                      BType_Bool_def,
+                                      bir_val_is_Bool_def,
+                                      bir_val_is_Imm_s_ALT_DEF,
+                                      bir_val_is_Imm_def,
+                                      bir_val_is_Unknown_def,
+                                      bir_val_is_Mem_def] >>
+METIS_TAC []
+);
 
 
 (* ------------------------------------------------------------------------- *)
@@ -226,15 +500,26 @@ REWRITE_TAC[bir_type_t_UNIV_SPEC, listTheory.FINITE_LIST_TO_SET]);
 (* ------------------------------------------------------------------------- *)
 
 val bir_default_value_of_type_def = Define `
-  (bir_default_value_of_type (BType_Imm s) = BVal_Imm (n2bs 0 s)) /\
-  (bir_default_value_of_type (BType_Mem a_s v_s) = BVal_Mem a_s v_s (FEMPTY))`;
+  (bir_default_value_of_type (BType_Imm s) =
+    BKVal_Imm (n2bs 0 s)
+  ) /\
+  (bir_default_value_of_type (BType_Mem a_s v_s) =
+    BKVal_Mem a_s v_s (FEMPTY)
+  )
+`;
 
-val bir_default_value_of_type_SPEC = store_thm ("bir_default_value_of_type_SPEC",
-  ``!ty. type_of_bir_val (bir_default_value_of_type ty) = SOME ty``,
+val bir_default_value_of_type_SPEC =
+  store_thm ("bir_default_value_of_type_SPEC",
+  ``!ty.
+      type_of_bir_val (BVal_Known (bir_default_value_of_type ty)) =
+         SOME ty``,
 
 Cases >> (
-  SIMP_TAC std_ss [bir_default_value_of_type_def, type_of_bir_val_def, type_of_n2bs]
-));
+  SIMP_TAC std_ss [bir_default_value_of_type_def,
+                   type_of_bir_val_def, type_of_bir_kval_def,
+                   type_of_n2bs]
+)
+);
 
 
 val _ = export_theory();
